ProofLibrary/SubstitutionAndHomomorphismBasics.lean
@@ -1,55 +1,58 @@
 import ProofLibrary.List
 import ProofLibrary.KnowledgeBaseBasics
 
-def GroundSubstitution := Variable -> GroundTerm
+section Defs
 
-def GroundTermMapping := GroundTerm -> GroundTerm
+  variable (sig : Signature) [DecidableEq sig.P] [DecidableEq sig.C] [DecidableEq sig.V]
+
+  abbrev GroundSubstitution := sig.V -> GroundTerm sig
+
+  abbrev GroundTermMapping := GroundTerm sig -> GroundTerm sig
+
+  class SubsTarget (α) (β) where
+    apply : GroundSubstitution sig -> α -> β
+
+
+end Defs
+
+
+variable {sig : Signature} [DecidableEq sig.P] [DecidableEq sig.C] [DecidableEq sig.V]
 
 namespace GroundSubstitution
-  def apply_var_or_const (σ : GroundSubstitution) : VarOrConst -> GroundTerm
+  def apply_var_or_const (σ : GroundSubstitution sig) : VarOrConst sig -> GroundTerm sig
     | .var v => σ v
     | .const c => GroundTerm.const c
 
-  def apply_skolem_term (σ : GroundSubstitution) : SkolemTerm -> GroundTerm
+  def apply_skolem_term (σ : GroundSubstitution sig) : SkolemTerm sig -> GroundTerm sig
     | .var v => σ v
     | .const c => GroundTerm.const c
-    | .func fs frontier => FiniteTree.inner fs (FiniteTreeList.fromList (frontier.map (fun fv => σ fv))) 
+    | .func fs frontier => FiniteTree.inner fs (FiniteTreeList.fromList (frontier.map (fun fv => σ fv)))
 
-  -- def apply_term (σ : GroundSubstitution) : Term -> GroundTerm
-  --   | .var v => σ v
-  --   | .const c => GroundTerm.const c
-  --   | .func ft => GroundTerm.func (FiniteTree.mapLeaves (fun voc => match voc with
-  --     | .var v => match σ v with
-  --       | .const c => FiniteTree.leaf c
-  --       | .func ft => ft
-  --     | .const c => FiniteTree.leaf c
-  --   ) ft)
-
-  def apply_atom (σ : GroundSubstitution) (ϕ : Atom) : Fact :=
+  def apply_atom (σ : GroundSubstitution sig) (ϕ : Atom sig) : Fact sig :=
     { predicate := ϕ.predicate, terms := List.map (apply_skolem_term σ) ϕ.terms }
 
-  def apply_function_free_atom (σ : GroundSubstitution) (ϕ : FunctionFreeAtom) : Fact :=
+  def apply_function_free_atom (σ : GroundSubstitution sig) (ϕ : FunctionFreeAtom sig) : Fact sig :=
     { predicate := ϕ.predicate, terms := List.map (apply_var_or_const σ) ϕ.terms }
 
-  def apply_function_free_conj (σ : GroundSubstitution) (conj : FunctionFreeConjunction) : List Fact :=
+  def apply_function_free_conj (σ : GroundSubstitution sig) (conj : FunctionFreeConjunction sig) : List (Fact sig) :=
     (List.map (apply_function_free_atom σ)) conj
 
-  theorem apply_same_length (σ : GroundSubstitution) (a : Atom) : a.terms.length = (σ.apply_atom a).terms.length := by 
+  theorem apply_same_length (σ : GroundSubstitution sig) (a : Atom sig) : a.terms.length = (σ.apply_atom a).terms.length := by
     simp [apply_atom]
 
-  theorem eq_under_subs_means_same_length (σ : GroundSubstitution) (a : Atom) (f : Fact) (h : σ.apply_atom a = f) : (a.terms.length = f.terms.length) := by 
+  theorem eq_under_subs_means_same_length (σ : GroundSubstitution sig) (a : Atom sig) (f : Fact sig) (h : σ.apply_atom a = f) : (a.terms.length = f.terms.length) := by
     rw [← h]
     simp [apply_atom]
 
-  theorem eq_under_subs_means_term_is_eq (σ : GroundSubstitution) (a : Atom) (f : Fact) (idx : Fin a.terms.length) (h : σ.apply_atom a = f) : (σ.apply_skolem_term (a.terms.get idx) = f.terms.get { val := idx.val, isLt := (by rw [← eq_under_subs_means_same_length σ a f h]; exact idx.isLt) }) := by
+  theorem eq_under_subs_means_term_is_eq (σ : GroundSubstitution sig) (a : Atom sig) (f : Fact sig) (idx : Fin a.terms.length) (h : σ.apply_atom a = f) : (σ.apply_skolem_term (a.terms.get idx) = f.terms.get { val := idx.val, isLt := (by rw [← eq_under_subs_means_same_length σ a f h]; exact idx.isLt) }) := by
     cases h
     simp [apply_atom]
 
   -- TODO: is the extra assumption with injectivity reasonable?
-  theorem eq_under_subs_means_elements_are_preserved [DecidableEq SkolemTerm] (σ : GroundSubstitution) (a : Atom) (f : Fact) (h : σ.apply_atom a = f) : ∀ t, (∀ s, s ∈ a.terms.toSet ∧ σ.apply_skolem_term t = σ.apply_skolem_term s -> t = s) -> ((σ.apply_skolem_term t) ∈ f.terms ↔ t ∈ a.terms) := by 
+  theorem eq_under_subs_means_elements_are_preserved (σ : GroundSubstitution sig) (a : Atom sig) (f : Fact sig) (h : σ.apply_atom a = f) : ∀ t, (∀ s, s ∈ a.terms.toSet ∧ σ.apply_skolem_term t = σ.apply_skolem_term s -> t = s) -> ((σ.apply_skolem_term t) ∈ f.terms ↔ t ∈ a.terms) := by
     intro t ht
-    rw [List.listElementIffToSetElement] 
-    rw [List.listElementIffToSetElement] 
+    rw [List.listElementIffToSetElement]
+    rw [List.listElementIffToSetElement]
     rw [← List.existsIndexIffInToSet]
     rw [← List.existsIndexIffInToSet]
     constructor
@@ -59,7 +62,7 @@ namespace GroundSubstitution
       rw [← eq_under_subs_means_term_is_eq σ a f j h] at hi
       apply ht
       constructor
-      . apply List.listGetInToSet 
+      . apply List.listGetInToSet
       . apply hi
     . intro ⟨i, hi⟩
       let j : Fin f.terms.length := ⟨i.val, (by rw [← eq_under_subs_means_same_length σ a f h]; exact i.isLt)⟩
@@ -68,7 +71,7 @@ namespace GroundSubstitution
       rw [hi]
 
   -- TODO: is the extra assumption with injectivity reasonable?
-  theorem eq_under_subs_means_indices_of_elements_are_preserved [DecidableEq SkolemTerm] (σ : GroundSubstitution) (a : Atom) (f : Fact) (h : σ.apply_atom a = f) (t : SkolemTerm) (ht : t ∈ a.terms) (hs : ∀ s, s ∈ a.terms.toSet ∧ σ.apply_skolem_term t = σ.apply_skolem_term s -> t = s) : (f.terms.idx_of (σ.apply_skolem_term t) (by rw [eq_under_subs_means_elements_are_preserved σ a f h t hs]; exact ht)).val = ((a.terms.idx_of t) ht).val := by 
+  theorem eq_under_subs_means_indices_of_elements_are_preserved (σ : GroundSubstitution sig) (a : Atom sig) (f : Fact sig) (h : σ.apply_atom a = f) (t : SkolemTerm sig) (ht : t ∈ a.terms) (hs : ∀ s, s ∈ a.terms.toSet ∧ σ.apply_skolem_term t = σ.apply_skolem_term s -> t = s) : (f.terms.idx_of (σ.apply_skolem_term t) (by rw [eq_under_subs_means_elements_are_preserved σ a f h t hs]; exact ht)).val = ((a.terms.idx_of t) ht).val := by
     have : f.terms = a.terms.map σ.apply_skolem_term := by rw [← h]; unfold apply_atom; simp
     rw [List.idx_of_eq_of_list_eq _ _ this _ _]
     apply Eq.symm
@@ -77,37 +80,38 @@ namespace GroundSubstitution
 
 end GroundSubstitution
 
-class SubsTarget (α) (β) where
-  apply : GroundSubstitution -> α -> β
-
-instance : SubsTarget SkolemTerm GroundTerm where
+instance : SubsTarget sig (SkolemTerm sig) (GroundTerm sig) where
   apply := GroundSubstitution.apply_skolem_term
 -- instance : SubsTarget Term GroundTerm where
 --   apply := GroundSubstitution.apply_term
-instance : SubsTarget Atom Fact where
+instance : SubsTarget sig (Atom sig) (Fact sig) where
   apply := GroundSubstitution.apply_atom
-instance : SubsTarget FunctionFreeAtom Fact where
+instance : SubsTarget sig (FunctionFreeAtom sig) (Fact sig) where
   apply := GroundSubstitution.apply_function_free_atom
-instance : SubsTarget FunctionFreeConjunction (List Fact) where
+instance : SubsTarget sig (FunctionFreeConjunction sig) (List (Fact sig)) where
   apply := GroundSubstitution.apply_function_free_conj
 
-def isIdOnConstants (h : GroundTermMapping) : Prop :=
-  ∀ t : GroundTerm, match t with
-    | GroundTerm.const _ => h t = t
-    | _ => True
+namespace GroundTermMapping
 
-def applyFact (h : GroundTermMapping) (f : Fact) : Fact :=
-  { predicate := f.predicate, terms := List.map h f.terms }
+  def isIdOnConstants (h : GroundTermMapping sig) : Prop :=
+    ∀ (t : GroundTerm sig), match t with
+      | GroundTerm.const _ => h t = t
+      | _ => True
 
-def applyFactSet (h : GroundTermMapping) (fs : FactSet) : FactSet :=
-  fun f' : Fact => ∃ f : Fact, (f ∈ fs) ∧ ((applyFact h f) = f')
+  def applyFact (h : GroundTermMapping sig) (f : Fact sig) : Fact sig :=
+    { predicate := f.predicate, terms := List.map h f.terms }
 
-def isHomomorphism (h : GroundTermMapping) (A B : FactSet) : Prop :=
-  isIdOnConstants h ∧ (applyFactSet h A ⊆ B)
+  def applyFactSet (h : GroundTermMapping sig) (fs : FactSet sig) : FactSet sig :=
+    fun f' : Fact sig => ∃ (f : Fact sig), (f ∈ fs) ∧ ((applyFact h f) = f')
 
-theorem applyPreservesElement (h : GroundTermMapping) (f : Fact) (fs : FactSet) : f ∈ fs -> applyFact h f ∈ applyFactSet h fs := by 
-  intro hf
-  simp [Set.element] at *
-  unfold applyFactSet
-  exists f
+  def isHomomorphism (h : GroundTermMapping sig) (A B : FactSet sig) : Prop :=
+    isIdOnConstants h ∧ (applyFactSet h A ⊆ B)
+
+  theorem applyPreservesElement (h : GroundTermMapping sig) (f : Fact sig) (fs : FactSet sig) : f ∈ fs -> applyFact h f ∈ applyFactSet h fs := by
+    intro hf
+    simp [Set.element] at *
+    unfold applyFactSet
+    exists f
+
+end GroundTermMapping
 
