ProofLibrary/TermBasics.lean
@@ -1,155 +1,96 @@
 import ProofLibrary.List
 import ProofLibrary.FiniteTree
 
-structure Predicate where
-  id : Nat
-  deriving DecidableEq
+structure Signature where
+  P : Type u
+  V : Type v
+  C : Type w
 
-structure Variable where
-  id : Nat
-  deriving DecidableEq
-
-structure Constant where
-  id : Nat
-  deriving DecidableEq
-
-/- I think we only need skolem function symbols
-structure FunctionSymbol where
-  id : Nat
--/
-
-structure SkolemFS where
+structure SkolemFS (sig : Signature) [DecidableEq sig.V] where
   ruleId : Nat
   disjunctIndex : Nat
-  var : Variable
+  var : sig.V
   deriving DecidableEq
 
--- inductive GroundTerm where
---   | const (c : Constant) : GroundTerm
---   | func (ft : FiniteTree SkolemFS Constant) : GroundTerm
---   deriving DecidableEq
+abbrev GroundTerm (sig : Signature) [DecidableEq sig.C] [DecidableEq sig.V] := FiniteTree (SkolemFS sig) sig.C
 
-def GroundTerm := FiniteTree SkolemFS Constant
-deriving DecidableEq
+inductive SkolemTerm (sig : Signature) [DecidableEq sig.C] [DecidableEq sig.V] where
+  | var (v : sig.V) : SkolemTerm sig
+  | const (c : sig.C) : SkolemTerm sig
+  | func (fs : SkolemFS sig) (frontier : List sig.V) : SkolemTerm sig
+  deriving DecidableEq
+
+inductive VarOrConst (sig : Signature) [DecidableEq sig.C] [DecidableEq sig.V] where
+  | var (v : sig.V) : VarOrConst sig
+  | const (c : sig.C) : VarOrConst sig
+  deriving DecidableEq
+
+variable {sig : Signature} [DecidableEq sig.C] [DecidableEq sig.V]
 
 @[match_pattern]
-def GroundTerm.const (c : Constant) := @FiniteTree.leaf SkolemFS Constant c
+def GroundTerm.const (c : sig.C) := @FiniteTree.leaf (SkolemFS sig) sig.C c
 
-inductive SkolemTerm where
-  | var (v : Variable) : SkolemTerm
-  | const (c : Constant) : SkolemTerm
-  | func (fs : SkolemFS) (frontier : List Variable) : SkolemTerm
-  deriving DecidableEq
-
-def SkolemTerm.variables : SkolemTerm -> List Variable
+def SkolemTerm.variables : SkolemTerm sig -> List sig.V
   | .var v => List.cons v List.nil
   | .const _ => List.nil
   | .func _ vs => vs
 
--- def GroundTerm.depth : GroundTerm -> Nat
---   | GroundTerm.const _ => 0
---   | GroundTerm.func ft => FiniteTree.depth ft
+namespace VarOrConst
 
-inductive VarOrConst where
-  | var (v : Variable) : VarOrConst
-  | const (c : Constant) : VarOrConst
-  deriving DecidableEq
+  def isVar : VarOrConst sig -> Bool
+  | .var _ => true
+  | .const _ => false
 
-def VarOrConst.isVar : VarOrConst -> Bool
-  | VarOrConst.var _ => true
-  | VarOrConst.const _ => false
+  def filterVars : List (VarOrConst sig) -> List sig.V
+  | .nil => List.nil
+  | .cons voc vocs => match voc with
+    | .var v => List.cons v (filterVars vocs)
+    | .const _ => (filterVars vocs)
 
-def VarOrConst.filterVars : List VarOrConst -> List Variable
-  | List.nil => List.nil
-  | List.cons voc vocs => match voc with
-    | VarOrConst.var v => List.cons v (VarOrConst.filterVars vocs)
-    | VarOrConst.const _ => (VarOrConst.filterVars vocs)
+  theorem filterVars_occur_in_original_list (l : List (VarOrConst sig)) (v : sig.V) : v ∈ (filterVars l).toSet -> VarOrConst.var v ∈ l.toSet := by
+    induction l with
+    | nil => intros; contradiction
+    | cons head tail ih =>
+      intro h
+      unfold filterVars at h
+      split at h
+      . simp [Set.element, List.toSet] at h
+        simp [Set.element, List.toSet]
+        cases h with
+        | inl hl => apply Or.inl; simp [Set.element] at hl; rw [hl]; simp [Set.element]
+        | inr hr => apply Or.inr; apply ih; apply hr
+      . simp [Set.element]
+        apply Or.inr
+        apply ih
+        apply h
 
-theorem VarOrConst.filterVars_occur_in_original_list (l : List VarOrConst) (v : Variable) : v ∈ (filterVars l).toSet -> VarOrConst.var v ∈ l.toSet := by
-  induction l with
-  | nil => intros; contradiction
-  | cons head tail ih =>
-    intro h
-    unfold filterVars at h
-    split at h
-    . simp [Set.element, List.toSet] at h
-      simp [Set.element, List.toSet]
-      cases h with
-      | inl hl => apply Or.inl; simp [Set.element] at hl; rw [hl]; simp [Set.element]
-      | inr hr => apply Or.inr; apply ih; apply hr
-    . simp [Set.element]
-      apply Or.inr
-      apply ih
-      apply h
+  def skolemize (ruleId : Nat) (disjunctIndex : Nat) (frontier : List sig.V) (voc : VarOrConst sig) : SkolemTerm sig :=
+    match voc with
+      | .var v => ite (v ∈ frontier)
+        (SkolemTerm.var v)
+        (SkolemTerm.func { ruleId, disjunctIndex, var := v} frontier)
+      | .const c => SkolemTerm.const c
 
--- inductive Term where
---   | var (v : Variable) : Term
---   | const (c : Constant) : Term
---   | func (ft : FiniteTree SkolemFS VarOrConst) : Term
---   deriving DecidableEq
---
--- def GroundTerm.toTerm : GroundTerm -> Term
---   | .const c => Term.const c
---   | .func ft => Term.func (FiniteTree.mapLeaves (fun c => FiniteTree.leaf (VarOrConst.const c)) ft)
---
--- instance : Coe GroundTerm Term where
---   coe := GroundTerm.toTerm
---
--- def SkolemTerm.toTerm : SkolemTerm -> Term
---   | .var v => Term.var v
---   | .const c => Term.const c
---   | .func fs frontier => Term.func (FiniteTree.inner fs (FiniteTreeList.fromList (frontier.map (fun fv => FiniteTree.leaf (VarOrConst.var fv)))))
---
--- instance : Coe SkolemTerm Term where
---   coe := SkolemTerm.toTerm
---
--- def Term.variables : Term -> List Variable
---   | Term.var v => List.cons v List.nil
---   | Term.const _ => List.nil
---   | Term.func ft => VarOrConst.filterVars ft.leaves
+  theorem skolemize_injective (ruleId : Nat) (disjunctIndex : Nat) (frontier : List sig.V) (s t : VarOrConst sig) : s.skolemize ruleId disjunctIndex frontier = t.skolemize ruleId disjunctIndex frontier -> s = t := by
+    cases s with
+    | var vs => cases t with
+      | var vt =>
+        simp [skolemize]
+        split
+        . split
+          . simp
+          . intros; contradiction
+        . split
+          . intros; contradiction
+          . simp
+      | const _ =>
+        simp only [skolemize]
+        split <;> intros <;> contradiction
+    | const cs => cases t with
+      | var vt =>
+        simp only [skolemize]
+        split <;> intros <;> contradiction
+      | const _ => simp [skolemize]
 
-def VarOrConst.skolemize (ruleId : Nat) (disjunctIndex : Nat) (frontier : List Variable) (voc : VarOrConst) : SkolemTerm :=
-  match voc with
-    | VarOrConst.var v => ite (v ∈ frontier)
-      (SkolemTerm.var v)
-      (SkolemTerm.func { ruleId, disjunctIndex, var := v} frontier)
-    | VarOrConst.const c => SkolemTerm.const c
-
-theorem VarOrConst.skolemize_injective (ruleId : Nat) (disjunctIndex : Nat) (frontier : List Variable) (s t : VarOrConst) : s.skolemize ruleId disjunctIndex frontier = t.skolemize ruleId disjunctIndex frontier -> s = t := by
-  cases s with
-  | var vs => cases t with
-    | var vt =>
-      simp [skolemize]
-      split
-      . split
-        . simp
-        . intros; contradiction
-      . split
-        . intros; contradiction
-        . simp
-    | const _ =>
-      simp only [skolemize]
-      split <;> intros <;> contradiction
-  | const cs => cases t with
-    | var vt =>
-      simp only [skolemize]
-      split <;> intros <;> contradiction
-    | const _ => simp [skolemize]
-
--- def VarOrConst.skolemize_into_functional_term (ruleId : Nat) (frontier : List Variable) (v : Variable) (v_not_frontier : ¬ frontier.elem v) : FiniteTree SkolemFS Variable :=
---   match eq : skolemize ruleId frontier (VarOrConst.var v) with
---   | .var _ => by simp [skolemize, v_not_frontier] at eq
---   | .const _ => by simp [skolemize, v_not_frontier] at eq
---   | .func ft =>
---     let mapper : VarOrConst
---     ft
---
--- theorem VarOrConst.skolemize_leaves_is_frontier (ruleId : Nat) (frontier : List Variable) (v : Variable) (v_not_frontier : ¬ frontier.elem v) : (skolemize_into_functional_term ruleId frontier v v_not_frontier).leaves = frontier := by sorry
-
--- def Term.skolemize (ruleId : Nat) (frontier : List Variable) (t : Term) : Term :=
---   match t with
---     | Term.var v => ite (List.elem v frontier)
---       (Term.var v)
---       (Term.func (FiniteTree.inner { ruleId := ruleId, var := v} (FiniteTreeList.fromList (List.map (fun fv => FiniteTree.leaf (VarOrConst.var fv)) frontier))))
---     | t => t
+end VarOrConst
 
