ProofLibrary/ChaseSequence/Universality.lean
@@ -1,0 +1,931 @@
+import ProofLibrary.ChaseSequence.Basic
+
+variable {sig : Signature} [DecidableEq sig.P] [DecidableEq sig.C] [DecidableEq sig.V]
+variable {obs : ObsoletenessCondition sig} {kb : KnowledgeBase sig}
+
+abbrev InductiveHomomorphismResult (ct : ChaseTree obs kb) (m : FactSet sig) (depth : Nat) := {pair : (List Nat) × (GroundTermMapping sig) // pair.1.length = depth ∧ (ct.tree.get pair.1).is_none_or (fun fs => pair.2.isHomomorphism fs.fact m) }
+
+-- TODO: split up the following definition (rather the proofs inside) to get rid of heartbeat increase
+set_option maxHeartbeats 1000000
+
+noncomputable def inductive_homomorphism_with_prev_node_and_trg (ct : ChaseTree obs kb) (m : FactSet sig) (m_is_model : m.modelsKb obs kb) (prev_depth : Nat) (prev_result : InductiveHomomorphismResult ct m prev_depth) (prev_node_unwrapped : ChaseNode obs kb.rules) (prev_node_eq : ct.tree.get prev_result.val.fst = some prev_node_unwrapped) (trg_ex : exists_trigger_list obs kb.rules prev_node_unwrapped (ct.tree.children prev_result.val.fst)) : InductiveHomomorphismResult ct m (prev_depth + 1) :=
+  let prev_path := prev_result.val.fst
+  let prev_hom := prev_result.val.snd
+  let prev_cond := prev_result.property
+  have prev_hom_is_homomorphism : prev_hom.isHomomorphism prev_node_unwrapped.fact m := by
+    have prev_cond_r := prev_cond.right
+    rw [prev_node_eq] at prev_cond_r
+    simp [Option.is_none_or] at prev_cond_r
+    exact prev_cond_r
+
+  let trg := Classical.choose trg_ex
+  let trg_spec := Classical.choose_spec trg_ex
+  let trg_active_for_current_step := trg_spec.left
+  let trg_result_used_for_next_chase_step := trg_spec.right
+
+  let trg_variant_for_m : RTrigger obs kb.rules := {
+    val := {
+      rule := trg.val.rule
+      subs := fun t => prev_hom (trg.val.subs t)
+    }
+    property := trg.property
+  }
+  have trg_variant_loaded_for_m : trg_variant_for_m.val.loaded m := by
+    have : trg_variant_for_m.val.loaded (prev_hom.applyFactSet prev_node_unwrapped.fact) := by
+      apply PreTrigger.term_mapping_preserves_loadedness
+      . exact prev_hom_is_homomorphism.left
+      . exact trg_active_for_current_step.left
+    apply Set.subsetTransitive
+    exact ⟨this, prev_hom_is_homomorphism.right⟩
+  have trg_variant_obsolete_on_m : obs.cond trg_variant_for_m.val m := by
+    have m_models_trg : m.modelsRule obs trg_variant_for_m.val.rule := by exact m_is_model.right trg.val.rule trg.property
+    unfold FactSet.modelsRule at m_models_trg
+    apply m_models_trg
+    constructor
+    rfl
+    apply trg_variant_loaded_for_m
+
+  let obs_for_m_subs := Classical.choose (obs.cond_implies_trg_is_satisfied trg_variant_obsolete_on_m)
+  let h_obs_for_m_subs := Classical.choose_spec (obs.cond_implies_trg_is_satisfied trg_variant_obsolete_on_m)
+  let head_index_for_m_subs := Classical.choose h_obs_for_m_subs
+  let h_obs_at_head_index_for_m_subs := Classical.choose_spec h_obs_for_m_subs
+
+  let result_index_for_trg : Fin trg.val.result.length := ⟨head_index_for_m_subs.val, by unfold PreTrigger.result; unfold PreTrigger.mapped_head; simp [List.enum_with_lt_length_eq]⟩
+
+  let next_hom : GroundTermMapping sig := fun t =>
+    match t with
+    | FiniteTree.leaf _ => t
+    | FiniteTree.inner _ _ =>
+      let t_in_step_j_dec := Classical.propDecidable (∃ f, f ∈ prev_node_unwrapped.fact.val ∧ t ∈ f.terms.toSet)
+      match t_in_step_j_dec with
+      | Decidable.isTrue _ => prev_hom t
+      | Decidable.isFalse _ =>
+        let t_in_trg_result_dec := Classical.propDecidable (∃ f, f ∈ (trg.val.result.get result_index_for_trg) ∧ t ∈ f.terms.toSet)
+        match t_in_trg_result_dec with
+        | Decidable.isFalse _ => t
+        | Decidable.isTrue t_in_trg_result =>
+          let f := Classical.choose t_in_trg_result
+          let ⟨f_in_trg_result, t_in_f⟩ := Classical.choose_spec t_in_trg_result
+
+          let idx_f := trg.val.idx_of_fact_in_result f result_index_for_trg f_in_trg_result
+          let atom_in_head := (trg.val.rule.head.get head_index_for_m_subs).get idx_f
+          let idx_t_in_f := f.terms.idx_of t (List.listToSetElementAlsoListElement _ _ t_in_f)
+          have idx_t_in_f_isLt := idx_t_in_f.isLt
+          have f_is_at_its_idx :
+            f = (trg.val.mapped_head.get ⟨head_index_for_m_subs.val, by simp [PreTrigger.mapped_head, List.enum_with_lt_length_eq]⟩).get ⟨idx_f.val, by simp [PreTrigger.mapped_head, List.enum_with_lt_getElem_snd_eq_getElem]⟩ := by simp [idx_f, PreTrigger.idx_of_fact_in_result]; apply List.idx_of_get
+
+          have atom_arity_same_as_fact : f.terms.length = List.length (FunctionFreeAtom.terms atom_in_head) := by
+              rw [f_is_at_its_idx]
+              unfold PreTrigger.mapped_head
+              unfold PreTrigger.apply_to_function_free_atom
+              simp [atom_in_head, List.enum_with_lt_getElem_snd_eq_getElem]
+
+          let term_corresponding_to_t := atom_in_head.terms.get ⟨idx_t_in_f.val, (by
+            rw [← atom_arity_same_as_fact]
+            exact idx_t_in_f_isLt
+          )⟩
+
+          obs_for_m_subs.apply_var_or_const term_corresponding_to_t
+
+  ⟨(head_index_for_m_subs.val::prev_path, next_hom), by
+    have prev_cond_r := prev_cond.right
+    rw [prev_node_eq] at prev_cond_r
+    simp [Option.is_none_or] at prev_cond_r
+
+    constructor
+    . simp; exact prev_cond.left
+    cases next_node_eq : ct.tree.get (head_index_for_m_subs.val::prev_path) with
+    | none => simp [Option.is_none_or]
+    | some next_node =>
+    simp only [Option.is_none_or]
+    constructor
+    . intro term
+      split
+      . simp
+      . trivial
+    have next_node_results_from_trg : next_node.fact = prev_node_unwrapped.fact ∪ trg.val.result.get result_index_for_trg := by
+      have length_eq_helper_1 : trg.val.rule.head.length = trg.val.result.enum_with_lt.attach.length := by
+        simp
+        rw [List.enum_with_lt_length_eq]
+        unfold PreTrigger.result
+        unfold PreTrigger.mapped_head
+        simp [List.enum_with_lt_length_eq]
+      have length_eq_helper_2 : trg_variant_for_m.val.rule.head.length = (ct.tree.children prev_path).length := by
+        rw [← trg_result_used_for_next_chase_step]
+        simp
+        simp at length_eq_helper_1
+        exact length_eq_helper_1
+      rw [List.map_eq_iff] at trg_result_used_for_next_chase_step
+      specialize trg_result_used_for_next_chase_step head_index_for_m_subs.val
+      have index_valid : head_index_for_m_subs < (ct.tree.children prev_path).length := by rw [← length_eq_helper_2]; exact head_index_for_m_subs.isLt
+      rw [List.getElem?_eq_getElem (l:=ct.tree.children prev_path) (n:=head_index_for_m_subs) index_valid] at trg_result_used_for_next_chase_step
+      rw [List.getElem?_eq_getElem (l:=trg.val.result.enum_with_lt.attach) (n:=head_index_for_m_subs) (by rw [← length_eq_helper_1]; simp)] at trg_result_used_for_next_chase_step
+      simp at trg_result_used_for_next_chase_step
+      have : some (ct.tree.children prev_path)[head_index_for_m_subs.val] = some next_node := by
+        rw [ct.tree.getElem_children_eq_get_tree prev_path ⟨head_index_for_m_subs.val, index_valid⟩]
+        exact next_node_eq
+      injection this with this
+      rw [this] at trg_result_used_for_next_chase_step
+      rw [trg_result_used_for_next_chase_step]
+      simp
+      rw [List.enum_with_lt_getElem_snd_eq_getElem]
+    rw [next_node_results_from_trg]
+
+    intro mapped_fact fact_in_chase
+
+    cases fact_in_chase with | intro fact fact_in_chase =>
+      rw [← fact_in_chase.right]
+      let fact_in_chase := fact_in_chase.left
+
+      cases fact_in_chase with
+      | inl fact_in_prev_step =>
+        apply prev_cond_r.right
+        exists fact
+        constructor
+        exact fact_in_prev_step
+        unfold GroundTermMapping.applyFact
+        simp
+        intro ground_term _
+        have : ∃ f, f ∈ prev_node_unwrapped.fact.val ∧ ground_term ∈ f.terms.toSet := by
+          exists fact
+          rw [← List.listElementIffToSetElement]
+          constructor
+          assumption
+          assumption
+        cases ground_term with
+        | leaf c => simp [next_hom]; apply prev_cond_r.left (GroundTerm.const c)
+        | inner _ _ =>
+          simp [next_hom]
+          split
+          . rfl
+          . contradiction
+      | inr fact_in_trg_result =>
+        let idx_of_fact_in_result := trg.val.idx_of_fact_in_result fact result_index_for_trg fact_in_trg_result
+        have fact_is_at_its_idx :
+          fact = (trg.val.mapped_head.get ⟨head_index_for_m_subs.val, by simp [PreTrigger.mapped_head, List.enum_with_lt_length_eq]⟩).get ⟨idx_of_fact_in_result.val, by simp [PreTrigger.mapped_head, List.enum_with_lt_getElem_snd_eq_getElem]⟩ := by simp [idx_of_fact_in_result, PreTrigger.idx_of_fact_in_result]; apply List.idx_of_get
+
+        rw [fact_is_at_its_idx]
+        unfold GroundTermMapping.applyFact
+
+        apply h_obs_at_head_index_for_m_subs.right
+        apply List.existsIndexMeansInToSet
+        exists ⟨idx_of_fact_in_result.val, (by
+          simp only [GroundSubstitution.apply_function_free_conj, List.length_map]
+          have isLt := idx_of_fact_in_result.isLt
+          simp only [List.get_eq_getElem, head_index_for_m_subs] at isLt
+          apply isLt
+        )⟩
+        simp only [GroundSubstitution.apply_function_free_conj, GroundSubstitution.apply_function_free_atom, PreTrigger.mapped_head, PreTrigger.apply_to_function_free_atom, List.get_eq_getElem, List.getElem_map]
+
+        -- we show that applying next_hom after trg is the same is applying trg_variant_for_m for each relevant VarOrConst
+
+        simp only [head_index_for_m_subs, Fact.mk.injEq]
+        constructor
+        . simp [List.enum_with_lt_getElem_snd_eq_getElem]
+        let head_disjunct : List (FunctionFreeAtom sig) := trg.val.rule.head[head_index_for_m_subs.val]
+        have : (trg.val.rule.head.enum[head_index_for_m_subs.val]'(by simp [List.enum_with_lt_length_eq])).snd = head_disjunct := by rw [List.getElem_enum]
+        have terms_eq : head_disjunct[idx_of_fact_in_result.val].terms = head_disjunct[idx_of_fact_in_result.val].terms := rfl
+        conv at terms_eq => left; simp only [← this]
+        conv at terms_eq => right; simp only [head_disjunct]
+        simp only [head_index_for_m_subs] at terms_eq
+        rw [List.map_map, terms_eq, List.map_eq_map_iff]
+        intro voc voc_is_in_head_atom_for_fact
+        cases voc with
+        | const _ => simp [PreTrigger.apply_to_var_or_const, PreTrigger.apply_to_skolemized_term, PreTrigger.skolemize_var_or_const, VarOrConst.skolemize, GroundSubstitution.apply_skolem_term, GroundSubstitution.apply_var_or_const]
+        | var v_from_head_atom =>
+          have : trg.val.rule.head.enum[head_index_for_m_subs.val].fst = head_index_for_m_subs.val := by simp
+          rw [this]
+          simp [next_hom, GroundSubstitution.apply_var_or_const]
+          split
+          case h_1 c h_c_eq =>
+            have v_is_in_frontier : v_from_head_atom ∈ trg.val.rule.frontier := by
+              apply Decidable.byContradiction
+              intro opp
+              simp [PreTrigger.apply_to_var_or_const, PreTrigger.apply_to_skolemized_term, PreTrigger.skolemize_var_or_const, GroundSubstitution.apply_skolem_term, VarOrConst.skolemize, opp] at h_c_eq
+            rw [h_obs_at_head_index_for_m_subs.left _ v_is_in_frontier]
+            simp [PreTrigger.apply_to_var_or_const, PreTrigger.apply_to_skolemized_term, PreTrigger.skolemize_var_or_const, GroundSubstitution.apply_skolem_term, VarOrConst.skolemize, v_is_in_frontier]
+            simp [PreTrigger.apply_to_var_or_const, PreTrigger.apply_to_skolemized_term, PreTrigger.skolemize_var_or_const, GroundSubstitution.apply_skolem_term, VarOrConst.skolemize, v_is_in_frontier] at h_c_eq
+            rw [h_c_eq]
+            have prev_hom_id_on_constants := prev_cond_r.left (FiniteTree.leaf c)
+            simp at prev_hom_id_on_constants
+            simp only [prev_hom]
+            rw [prev_hom_id_on_constants]
+          case h_2 =>
+            split
+            case h_1 _ exis_f _ =>
+              have v_is_in_frontier : v_from_head_atom ∈ trg.val.rule.frontier := by
+                apply Decidable.byContradiction
+                intro v_not_in_frontier
+                simp at v_not_in_frontier
+
+                have : (trg.val.result.get result_index_for_trg) ⊆ prev_node_unwrapped.fact := by
+                  apply funcTermForExisVarInChaseMeansTriggerResultOccurs ct trg result_index_for_trg v_from_head_atom prev_node_unwrapped prev_path
+                  constructor
+                  . rw [prev_node_eq]
+                  constructor
+                  . apply v_not_in_frontier
+                  . simp [result_index_for_trg]
+                    apply exis_f
+
+                have : obs.cond trg.val prev_node_unwrapped.fact := obs.contains_trg_result_implies_cond result_index_for_trg this
+                have : ¬ obs.cond trg.val prev_node_unwrapped.fact := trg_active_for_current_step.right
+                contradiction
+
+              rw [h_obs_at_head_index_for_m_subs.left]
+              simp [PreTrigger.apply_to_var_or_const, PreTrigger.apply_to_skolemized_term, PreTrigger.skolemize_var_or_const, GroundSubstitution.apply_skolem_term, VarOrConst.skolemize, v_is_in_frontier]
+              have : trg.val.rule = trg_variant_for_m.val.rule := by rfl
+              rw [← this]
+              apply v_is_in_frontier
+            case h_2 _ n_exis_f_for_step_j _ =>
+              have v_not_in_frontier : ¬ v_from_head_atom ∈ trg.val.rule.frontier := by
+                intro v_is_in_frontier
+                have v_in_body := Rule.frontier_var_occurs_in_fact_in_body _ _ v_is_in_frontier
+                cases v_in_body with | intro f hf =>
+                  apply n_exis_f_for_step_j
+                  exists (trg.val.subs.apply_function_free_atom f)
+                  constructor
+                  . apply trg_active_for_current_step.left
+                    unfold PreTrigger.mapped_body
+                    apply List.mappedElemInMappedList
+                    apply hf.left
+                  . simp [PreTrigger.apply_to_var_or_const, PreTrigger.apply_to_skolemized_term, PreTrigger.skolemize_var_or_const, GroundSubstitution.apply_skolem_term, VarOrConst.skolemize, v_is_in_frontier, GroundSubstitution.apply_function_free_atom]
+                    have : trg.val.subs v_from_head_atom = trg.val.subs.apply_var_or_const (VarOrConst.var v_from_head_atom) := by simp [GroundSubstitution.apply_var_or_const]
+                    rw [this]
+                    apply List.mappedElemInMappedList
+                    apply hf.right
+              split
+              case h_1 _ n_exis_f_for_trg_result _ =>
+                apply False.elim
+                apply n_exis_f_for_trg_result
+                exists fact
+                constructor
+                . exact fact_in_trg_result
+                rw [fact_is_at_its_idx]
+
+                rw [← PreTrigger.apply_subs_to_atom_at_idx_same_as_fact_at_idx]
+
+                apply List.existsIndexMeansInToSet
+                rw [List.listElementIffToSetElement] at voc_is_in_head_atom_for_fact
+                cases (List.inToSetMeansExistsIndex _ _ voc_is_in_head_atom_for_fact) with | intro voc_idx h_voc_idx =>
+                  exists ⟨voc_idx.val, (by
+                    rw [← PreTrigger.apply_to_function_free_atom_terms_same_length]
+                    apply voc_idx.isLt
+                  )⟩
+                  simp only [GroundSubstitution.apply_atom, VarOrConst.skolemize, GroundSubstitution.apply_skolem_term, FunctionFreeAtom.skolemize, PreTrigger.apply_to_function_free_atom, PreTrigger.apply_to_var_or_const, PreTrigger.apply_to_skolemized_term, PreTrigger.skolemize_var_or_const]
+                  simp only [List.get_eq_getElem, List.getElem_map, head_index_for_m_subs]
+                  simp only [List.get_eq_getElem] at h_voc_idx
+                  rw [← h_voc_idx]
+              case h_2 _ exis_f _ =>
+                split
+                case _ _ chosen_f_in_result applied_v_is_in_chosen_f _ =>
+                  let v_from_head_atom := VarOrConst.var v_from_head_atom
+                  let skolem_v := trg.val.skolemize_var_or_const head_index_for_m_subs v_from_head_atom
+                  let chosen_f := Classical.choose exis_f
+
+                  let idx_f := trg.val.idx_of_fact_in_result chosen_f result_index_for_trg chosen_f_in_result
+                  let atom_in_head := (trg.val.rule.head.get head_index_for_m_subs).get idx_f
+                  let idx_v_in_f := chosen_f.terms.idx_of (trg.val.apply_to_var_or_const head_index_for_m_subs v_from_head_atom) (List.listToSetElementAlsoListElement _ _ applied_v_is_in_chosen_f)
+                  have idx_v_in_f_isLt := idx_v_in_f.isLt
+                  have f_is_at_its_idx : chosen_f = (trg.val.mapped_head.get ⟨head_index_for_m_subs.val, by simp [PreTrigger.mapped_head, List.enum_with_lt_length_eq]⟩).get ⟨idx_f.val, by simp [PreTrigger.mapped_head, List.enum_with_lt_getElem_snd_eq_getElem]⟩ := by simp [idx_f, PreTrigger.idx_of_fact_in_result]; apply List.idx_of_get
+                  have v_is_at_its_idx : (trg.val.apply_to_var_or_const head_index_for_m_subs v_from_head_atom) = chosen_f.terms.get idx_v_in_f := by simp [idx_v_in_f]; apply List.idx_of_get
+
+                  have atom_arity_same_as_fact : chosen_f.terms.length = List.length (FunctionFreeAtom.terms atom_in_head) := by
+                    rw [f_is_at_its_idx]
+                    unfold PreTrigger.mapped_head
+                    simp
+                    rw [← PreTrigger.apply_to_function_free_atom_terms_same_length]
+                    simp [atom_in_head, List.enum_with_lt_getElem_snd_eq_getElem]
+
+                  let var_corresponding_to_applied_v := atom_in_head.terms.get ⟨idx_v_in_f.val, (by
+                    rw [← atom_arity_same_as_fact]
+                    exact idx_v_in_f_isLt
+                  )⟩
+
+                  let skolem_term_corresponding_to_applied_v := trg.val.skolemize_var_or_const head_index_for_m_subs var_corresponding_to_applied_v
+
+                  have subs_application_is_injective_for_freshly_introduced_terms : ∀ s, trg.val.apply_to_skolemized_term skolem_v = trg.val.apply_to_var_or_const head_index_for_m_subs s -> skolem_v = trg.val.skolemize_var_or_const head_index_for_m_subs s := by
+                    intro s hs
+                    cases s with
+                    | const const_s =>
+                      simp [skolem_v, PreTrigger.apply_to_var_or_const, PreTrigger.apply_to_skolemized_term, PreTrigger.skolemize_var_or_const, VarOrConst.skolemize, v_not_in_frontier, GroundSubstitution.apply_skolem_term] at hs
+                      contradiction
+                    | var var_s =>
+                      apply PreTrigger.subs_application_is_injective_for_freshly_introduced_terms
+                      apply v_not_in_frontier
+                      apply hs
+
+                  have skolemized_ts_are_equal : skolem_term_corresponding_to_applied_v = skolem_v := by
+                    apply Eq.symm
+                    apply subs_application_is_injective_for_freshly_introduced_terms
+                    unfold PreTrigger.apply_to_var_or_const at v_is_at_its_idx
+                    simp at v_is_at_its_idx
+                    rw [v_is_at_its_idx]
+
+                    have : chosen_f.terms = (trg.val.apply_to_function_free_atom head_index_for_m_subs atom_in_head).terms := by
+                      rw [f_is_at_its_idx]
+                      rw [← PreTrigger.apply_subs_to_atom_at_idx_same_as_fact_at_idx]
+
+                    simp [this, PreTrigger.apply_to_function_free_atom, var_corresponding_to_applied_v]
+
+                  have : var_corresponding_to_applied_v = v_from_head_atom := by
+                    apply VarOrConst.skolemize_injective trg.val.rule.id head_index_for_m_subs (Rule.frontier trg.val.rule)
+                    apply skolemized_ts_are_equal
+
+                  simp [var_corresponding_to_applied_v, atom_in_head] at this
+                  rw [this]
+  ⟩
+
+noncomputable def inductive_homomorphism_with_prev_node (ct : ChaseTree obs kb) (m : FactSet sig) (m_is_model : m.modelsKb obs kb) (prev_depth : Nat) (prev_result : InductiveHomomorphismResult ct m prev_depth) (prev_node_unwrapped : ChaseNode obs kb.rules) (prev_node_eq : ct.tree.get prev_result.val.fst = some prev_node_unwrapped) : InductiveHomomorphismResult ct m (prev_depth + 1) :=
+  let trg_ex_dec := Classical.propDecidable (exists_trigger_list obs kb.rules prev_node_unwrapped (ct.tree.children prev_result.val.fst))
+  match trg_ex_dec with
+  | .isFalse _ =>
+    let ⟨(prev_path, prev_hom), prev_cond⟩ := prev_result
+    -- just prepending zero here as it does not really matter which index we append but the length must match
+    ⟨(0::prev_path, prev_hom), by
+      constructor
+      . simp; exact prev_cond.left
+      . have : ct.tree.get (0::prev_path) = none := by
+          apply FiniteDegreeTree.children_empty_means_all_following_none
+          let triggers_exist := ct.triggers_exist prev_path
+          rw [prev_node_eq] at triggers_exist
+          simp [Option.is_none_or] at triggers_exist
+          cases triggers_exist with
+          | inl _ => contradiction
+          | inr hr => unfold not_exists_trigger_list at hr; exact hr.right
+        rw [this]
+        simp [Option.is_none_or]
+    ⟩
+  | .isTrue trg_ex =>
+    inductive_homomorphism_with_prev_node_and_trg ct m m_is_model prev_depth prev_result prev_node_unwrapped prev_node_eq trg_ex
+
+noncomputable def inductive_homomorphism (ct : ChaseTree obs kb) (m : FactSet sig) (m_is_model : m.modelsKb obs kb) : (depth : Nat) ->
+  InductiveHomomorphismResult ct m depth
+| .zero => ⟨([], id), by
+  simp [Option.is_none_or]; rw [ct.database_first]; simp
+  constructor
+  . unfold GroundTermMapping.isIdOnConstants; intro gt ; cases gt <;> simp
+  . intro el
+    simp [Set.element]
+    intro el_in_set
+    cases el_in_set with | intro f hf =>
+      apply m_is_model.left
+      simp [Set.element]
+      have : f = el := by have hfr := hf.right; simp [GroundTermMapping.applyFact, List.map_id'] at hfr; exact hfr
+      rw [this] at hf
+      exact hf.left
+⟩
+| .succ j =>
+  let ⟨(prev_path, prev_hom), prev_cond⟩ := inductive_homomorphism ct m m_is_model j
+  let prev_node := ct.tree.get prev_path
+
+  match prev_node_eq : prev_node with
+  | .none =>
+    -- just prepending zero here as it does not really matter which index we append but the length must match
+    ⟨(0::prev_path, prev_hom), by
+      constructor
+      . simp; exact prev_cond.left
+      . have : ct.tree.get (0::prev_path) = none := by
+          apply Option.decidable_eq_none.byContradiction
+          intro contra
+          apply ct.tree.tree.no_orphans _ contra ⟨prev_path, by exists [0]⟩
+          simp [prev_node] at prev_node_eq
+          unfold FiniteDegreeTree.get at prev_node_eq
+          unfold PossiblyInfiniteTree.get at prev_node_eq
+          simp
+          exact prev_node_eq
+        rw [this]
+        simp [Option.is_none_or]
+    ⟩
+  | .some prev_node_unwrapped =>
+    inductive_homomorphism_with_prev_node ct m m_is_model j ⟨⟨prev_path, prev_hom⟩, prev_cond⟩ prev_node_unwrapped prev_node_eq
+termination_by depth => depth
+
+theorem inductive_homomorphism_with_prev_node_and_trg_path_not_empty (ct : ChaseTree obs kb) (m : FactSet sig) (m_is_model : m.modelsKb obs kb) (prev_depth : Nat) (prev_result : InductiveHomomorphismResult ct m prev_depth) (prev_node_unwrapped : ChaseNode obs kb.rules) (prev_node_eq : ct.tree.get prev_result.val.fst = some prev_node_unwrapped) (trg_ex : exists_trigger_list obs kb.rules prev_node_unwrapped (ct.tree.children prev_result.val.fst)) : (inductive_homomorphism_with_prev_node_and_trg ct m m_is_model prev_depth prev_result prev_node_unwrapped prev_node_eq trg_ex).val.1 ≠ [] := by
+  unfold inductive_homomorphism_with_prev_node_and_trg
+  simp
+
+theorem inductive_homomorphism_path_not_empty {ct : ChaseTree obs kb} : ∀ n, (inductive_homomorphism ct m m_is_model (n+1)).val.1 ≠ [] := by
+  intro n
+  unfold inductive_homomorphism
+  split
+  simp
+  split
+  . simp
+  unfold inductive_homomorphism_with_prev_node
+  simp
+  split
+  . simp
+  apply inductive_homomorphism_with_prev_node_and_trg_path_not_empty
+
+theorem inductive_homomorphism_with_prev_node_and_trg_path_extends_prev (ct : ChaseTree obs kb) (m : FactSet sig) (m_is_model : m.modelsKb obs kb) (prev_depth : Nat) (prev_result : InductiveHomomorphismResult ct m prev_depth) (prev_node_unwrapped : ChaseNode obs kb.rules) (prev_node_eq : ct.tree.get prev_result.val.fst = some prev_node_unwrapped) (trg_ex : exists_trigger_list obs kb.rules prev_node_unwrapped (ct.tree.children prev_result.val.fst)) : (inductive_homomorphism_with_prev_node_and_trg ct m m_is_model prev_depth prev_result prev_node_unwrapped prev_node_eq trg_ex).val.1 = ((inductive_homomorphism_with_prev_node_and_trg ct m m_is_model prev_depth prev_result prev_node_unwrapped prev_node_eq trg_ex).val.1.head (by apply inductive_homomorphism_with_prev_node_and_trg_path_not_empty)) :: prev_result.val.fst := by
+  conv => left; rw [List.head_cons_tail _ (inductive_homomorphism_with_prev_node_and_trg_path_not_empty ct m m_is_model prev_depth prev_result prev_node_unwrapped prev_node_eq trg_ex)]
+  simp
+  unfold inductive_homomorphism_with_prev_node_and_trg
+  simp
+
+theorem inductive_homomorphism_path_extends_prev {ct : ChaseTree obs kb} : ∀ n, (inductive_homomorphism ct m m_is_model (n+1)).val.1 = ((inductive_homomorphism ct m m_is_model (n+1)).val.1.head (by apply inductive_homomorphism_path_not_empty)) :: (inductive_homomorphism ct m m_is_model n).val.1 := by
+  intro n
+  conv => left; rw [List.head_cons_tail _ (inductive_homomorphism_path_not_empty n)]
+  simp
+  conv => left; unfold inductive_homomorphism
+  split
+  case _ prev_path _ _ heq =>
+    have : prev_path = (inductive_homomorphism ct m m_is_model n).val.1 := by rw [heq]
+    simp
+    split
+    . simp; exact this
+    unfold inductive_homomorphism_with_prev_node
+    simp
+    split
+    . simp; exact this
+    unfold inductive_homomorphism_with_prev_node_and_trg
+    simp; exact this
+
+theorem inductive_homomorphism_path_extends_all_prev {ct : ChaseTree obs kb} : ∀ n d, (inductive_homomorphism ct m m_is_model (n+d)).val.1 = ((inductive_homomorphism ct m m_is_model (n+d)).val.1.take d) ++ (inductive_homomorphism ct m m_is_model n).val.1 := by
+  intro n d
+  induction d with
+  | zero => simp
+  | succ d ih =>
+    rw [← Nat.add_assoc]
+    rw [inductive_homomorphism_path_extends_prev (n+d)]
+    simp
+    exact ih
+
+theorem inductive_homomorphism_with_prev_node_and_trg_latest_index_lt_trg_result_length
+  {ct : ChaseTree obs kb}
+  (prev_step : Nat)
+  (prev_node : ChaseNode obs kb.rules)
+  (prev_ex : some prev_node = ct.tree.get (inductive_homomorphism ct m m_is_model prev_step).val.1)
+  (trg_ex : exists_trigger_list obs kb.rules prev_node (ct.tree.children (inductive_homomorphism ct m m_is_model prev_step).val.1))
+  : (inductive_homomorphism_with_prev_node_and_trg ct m m_is_model prev_step _ _ (Eq.symm prev_ex) trg_ex).val.1.head (by apply inductive_homomorphism_with_prev_node_and_trg_path_not_empty) < (Classical.choose trg_ex).val.result.length := by
+    let prev_result := inductive_homomorphism ct m m_is_model prev_step
+    let prev_hom := prev_result.val.snd
+    let prev_cond := prev_result.property
+    have prev_hom_is_homomorphism : prev_hom.isHomomorphism prev_node.fact m := by
+      have prev_cond_r := prev_cond.right
+      simp only [prev_result] at prev_cond_r
+      rw [← prev_ex] at prev_cond_r
+      simp [Option.is_none_or] at prev_cond_r
+      exact prev_cond_r
+
+    let trg := Classical.choose trg_ex
+    let trg_spec := Classical.choose_spec trg_ex
+    let trg_active_for_current_step := trg_spec.left
+
+    let trg_variant_for_m : RTrigger obs kb.rules := {
+      val := {
+        rule := trg.val.rule
+        subs := fun t => prev_hom (trg.val.subs t)
+      }
+      property := trg.property
+    }
+    have trg_variant_loaded_for_m : trg_variant_for_m.val.loaded m := by
+      have : trg_variant_for_m.val.loaded (prev_hom.applyFactSet prev_node.fact) := by
+        apply PreTrigger.term_mapping_preserves_loadedness
+        . exact prev_hom_is_homomorphism.left
+        . exact trg_active_for_current_step.left
+      apply Set.subsetTransitive
+      exact ⟨this, prev_hom_is_homomorphism.right⟩
+    have trg_variant_obsolete_on_m : obs.cond trg_variant_for_m.val m := by
+      have m_models_trg : m.modelsRule obs trg_variant_for_m.val.rule := by exact m_is_model.right trg.val.rule trg.property
+      unfold FactSet.modelsRule at m_models_trg
+      apply m_models_trg
+      constructor
+      rfl
+      apply trg_variant_loaded_for_m
+
+    let h_obs_for_m_subs := Classical.choose_spec (obs.cond_implies_trg_is_satisfied trg_variant_obsolete_on_m)
+    let head_index_for_m_subs := Classical.choose h_obs_for_m_subs
+
+    have : (inductive_homomorphism_with_prev_node_and_trg ct m m_is_model prev_step (inductive_homomorphism ct m m_is_model prev_step) prev_node (by rw [prev_ex]) trg_ex).val.fst = head_index_for_m_subs.val :: prev_result.val.fst := by
+      unfold inductive_homomorphism_with_prev_node_and_trg
+      simp [head_index_for_m_subs]
+    simp [this]
+    have isLt := head_index_for_m_subs.isLt
+    simp only [trg_variant_for_m, trg] at isLt
+    unfold PreTrigger.result
+    simp only [PreTrigger.head_length_eq_mapped_head_length] at isLt
+    simp
+    exact isLt
+
+theorem inductive_homomorphism_latest_index_lt_trg_result_length
+  {ct : ChaseTree obs kb}
+  (prev_step : Nat)
+  (prev_node : ChaseNode obs kb.rules)
+  (prev_ex : some prev_node = ct.tree.get (inductive_homomorphism ct m m_is_model prev_step).val.1)
+  (trg_ex : exists_trigger_list obs kb.rules prev_node (ct.tree.children (inductive_homomorphism ct m m_is_model prev_step).val.1))
+  : (inductive_homomorphism ct m m_is_model (prev_step+1)).val.1.head (by apply inductive_homomorphism_path_not_empty) < (Classical.choose trg_ex).val.result.length := by
+
+    have : inductive_homomorphism ct m m_is_model (prev_step + 1) = inductive_homomorphism_with_prev_node ct m m_is_model prev_step (inductive_homomorphism ct m m_is_model prev_step) prev_node (by rw [prev_ex]) := by
+      conv => left; unfold inductive_homomorphism
+      simp
+      split
+      case h_1 heq => rw [heq] at prev_ex; contradiction
+      case h_2 heq =>
+        rw [heq] at prev_ex
+        injection prev_ex with prev_ex
+        simp [← prev_ex]
+    simp [this]
+
+    have : inductive_homomorphism_with_prev_node ct m m_is_model prev_step (inductive_homomorphism ct m m_is_model prev_step) prev_node (by rw [prev_ex]) = inductive_homomorphism_with_prev_node_and_trg ct m m_is_model prev_step (inductive_homomorphism ct m m_is_model prev_step) prev_node (Eq.symm prev_ex) trg_ex := by
+      conv => left; unfold inductive_homomorphism_with_prev_node
+      simp
+      split
+      case h_1 _ h _ => apply False.elim; apply h; apply trg_ex
+      case h_2 => simp
+    simp [this]
+
+    apply inductive_homomorphism_with_prev_node_and_trg_latest_index_lt_trg_result_length
+    exact prev_ex
+
+theorem inductive_homomorphism_tree_get_path_none_means_layer_empty {ct : ChaseTree obs kb} : ∀ n, ct.tree.get (inductive_homomorphism ct m m_is_model (n+1)).val.fst = none -> ct.tree.children (inductive_homomorphism ct m m_is_model n).val.fst = [] := by
+  intro n succ_none
+  unfold inductive_homomorphism at succ_none
+  simp at succ_none
+  split at succ_none
+  . simp at succ_none; apply ct.tree.first_child_none_means_children_empty; exact succ_none
+  case h_2 _ heq =>
+    unfold inductive_homomorphism_with_prev_node at succ_none
+    simp at succ_none
+    split at succ_none
+    . simp at succ_none; apply ct.tree.first_child_none_means_children_empty; exact succ_none
+    case h_2 _ ex _ =>
+      let child_index : Fin (ct.tree.children (inductive_homomorphism ct m m_is_model n).val.fst).length := ⟨
+        (inductive_homomorphism_with_prev_node_and_trg ct m m_is_model n _ _ heq ex).val.1.head (by apply inductive_homomorphism_with_prev_node_and_trg_path_not_empty),
+        by
+          let trg_spec := Classical.choose_spec ex
+          rw [← trg_spec.right]
+          simp
+          rw [List.enum_with_lt_length_eq]
+          apply inductive_homomorphism_with_prev_node_and_trg_latest_index_lt_trg_result_length
+          rw [heq]
+      ⟩
+
+      let child := (ct.tree.children (inductive_homomorphism ct m m_is_model n).val.fst)[child_index.val]
+      have : some child = ct.tree.get (inductive_homomorphism_with_prev_node_and_trg ct m m_is_model n _ _ heq ex).val.fst := by
+        simp only [child]
+        rw [ct.tree.getElem_children_eq_get_tree _ child_index]
+        have : child_index.val :: (inductive_homomorphism ct m m_is_model n).val.fst = (inductive_homomorphism_with_prev_node_and_trg ct m m_is_model n _ _ heq ex).val.fst := by rw [inductive_homomorphism_with_prev_node_and_trg_path_extends_prev]
+        rw [this]
+
+      rw [← this] at succ_none
+      contradiction
+
+theorem inductive_homomorphism_same_on_terms_in_next_step (ct : ChaseTree obs kb) (m : FactSet sig) (m_is_model : m.modelsKb obs kb) : ∀ i, (ct.tree.get (inductive_homomorphism ct m m_is_model i).val.fst).is_none_or (fun node => ∀ f t, f ∈ node.fact.val ∧ t ∈ f.terms.toSet -> (inductive_homomorphism ct m m_is_model i).val.snd t = (inductive_homomorphism ct m m_is_model i.succ).val.snd t) := by
+  intro i
+  cases eq : ct.tree.get (inductive_homomorphism ct m m_is_model i).val.fst with
+  | none => simp [Option.is_none_or]
+  | some node =>
+    intro f t precondition
+    conv => rhs; unfold inductive_homomorphism; simp
+    split
+    case h_1 _ => simp
+    case h_2 heq =>
+      unfold inductive_homomorphism_with_prev_node
+      simp
+      split
+      . simp
+      . unfold inductive_homomorphism_with_prev_node_and_trg
+        simp
+        split
+        case h_1 c =>
+          have property := (inductive_homomorphism ct m m_is_model i).property.right
+          rw [eq] at property; simp [Option.is_none_or] at property
+          exact property.left (GroundTerm.const c)
+        case h_2 ft =>
+          split
+          case h_1 _ ex_f _ => rfl
+          case h_2 _ n_ex_f _ =>
+            apply False.elim; apply n_ex_f; exists f; constructor
+            . rw [heq] at eq; injection eq with eq; rw [eq]; exact precondition.left
+            . exact precondition.right
+
+theorem inductive_homomorphism_same_on_all_following_terms (ct : ChaseTree obs kb) (m : FactSet sig) (m_is_model : m.modelsKb obs kb) : ∀ i, (ct.tree.get (inductive_homomorphism ct m m_is_model i).val.fst).is_none_or (fun node => ∀ j f t, f ∈ node.fact.val ∧ t ∈ f.terms.toSet -> (inductive_homomorphism ct m m_is_model i).val.snd t = (inductive_homomorphism ct m m_is_model (i+j)).val.snd t) := by
+  intro i
+  cases eq : ct.tree.get (inductive_homomorphism ct m m_is_model i).val.fst with
+  | none => simp [Option.is_none_or]
+  | some node =>
+    intro j f t
+    induction j with
+    | zero => intros; rfl
+    | succ j ih =>
+      intro precond
+      rw [ih precond]
+      have next_step := inductive_homomorphism_same_on_terms_in_next_step ct m m_is_model (i + j)
+      cases eq2 : ct.tree.get (inductive_homomorphism ct m m_is_model (i+j)).val.fst with
+      | none =>
+        conv => right; unfold inductive_homomorphism
+        simp
+        split
+        case h_1 _ => simp
+        case h_2 heq => rw [heq] at eq2; contradiction
+      | some node2 =>
+        rw [eq2] at next_step; simp [Option.is_none_or] at next_step
+        specialize next_step f t
+        apply next_step
+        . have subset_following := chaseTreeSetIsSubsetOfAllFollowing ct (inductive_homomorphism ct m m_is_model i).val.fst ((inductive_homomorphism ct m m_is_model (i+j)).val.fst.take j)
+          rw [eq] at subset_following
+          simp at subset_following
+          rw [← inductive_homomorphism_path_extends_all_prev i j] at subset_following
+          rw [eq2] at subset_following
+          simp [Option.is_none_or] at subset_following
+          apply subset_following
+          exact precond.left
+        . exact precond.right
+
+theorem chaseTreeResultIsUniversal (ct : ChaseTree obs kb) : ∀ (m : FactSet sig), m.modelsKb obs kb -> ∃ (fs : FactSet sig) (h : GroundTermMapping sig), fs ∈ ct.result ∧ h.isHomomorphism fs m := by
+  intro m m_is_model
+
+  let inductive_homomorphism_shortcut := inductive_homomorphism ct m m_is_model
+
+  let indices : InfiniteList Nat := fun n => (inductive_homomorphism_shortcut (n + 1)).val.1.head (by apply inductive_homomorphism_path_not_empty)
+
+  have indices_aux_result : ∀ n, (indices.take n).reverse = (inductive_homomorphism_shortcut n).val.1 := by
+    intro n
+    induction n with
+    | zero =>
+      simp [inductive_homomorphism_shortcut]
+      unfold inductive_homomorphism
+      unfold InfiniteList.take
+      simp
+    | succ n ih =>
+      unfold InfiniteList.take
+      rw [List.reverse_append]
+      simp
+      rw [inductive_homomorphism_path_extends_prev]
+      simp
+      exact ih
+
+  let path : Nat -> Option (ChaseNode obs kb.rules) := fun n => (ct.tree.get (inductive_homomorphism_shortcut n).val.1)
+  let nodes : PossiblyInfiniteList (ChaseNode obs kb.rules) := {
+    infinite_list := path
+    no_holes := by
+      intro n path_not_none m
+      simp only [path]
+      simp only [path] at path_not_none
+      unfold FiniteDegreeTree.get at path_not_none
+      unfold PossiblyInfiniteTree.get at path_not_none
+      have no_orphans := ct.tree.tree.no_orphans
+        (inductive_homomorphism_shortcut n).val.1
+        path_not_none
+        ⟨(inductive_homomorphism_shortcut m).val.1, by
+          exists ((indices.skip m).take (n - m)).reverse
+          rw [← indices_aux_result m]
+          rw [← List.reverse_append]
+          rw [InfiniteList.combine_skip_take]
+          exact indices_aux_result n
+        ⟩
+      exact no_orphans
+  }
+  let branch : ChaseBranch obs kb := {
+    branch := nodes
+    database_first := by
+      simp only [nodes, path, inductive_homomorphism_shortcut]
+      unfold inductive_homomorphism
+      simp
+      rw [ct.database_first]
+    triggers_exist := by
+      intro n
+      cases eq : nodes.infinite_list n with
+      | none => simp [Option.is_none_or]
+      | some node =>
+        simp [Option.is_none_or]
+        simp only [nodes, path]
+        simp only [nodes, path] at eq
+        have ex_trg := ct.triggers_exist (inductive_homomorphism_shortcut n).val.1
+        rw [eq] at ex_trg
+        simp [Option.is_none_or] at ex_trg
+        cases ex_trg with
+        | inl ex_trg =>
+          apply Or.inl
+          unfold exists_trigger_opt_fs
+          unfold exists_trigger_list at ex_trg
+          let trg := Classical.choose ex_trg
+          let h := Classical.choose_spec ex_trg
+          exists trg
+          constructor
+          . exact h.left
+          let i : Fin trg.val.result.length := ⟨((inductive_homomorphism_shortcut (n+1)).val.fst.head (inductive_homomorphism_path_not_empty n)), inductive_homomorphism_latest_index_lt_trg_result_length n node (by rw [← eq]) ex_trg⟩
+          let i' : Fin (ct.tree.children (inductive_homomorphism_shortcut n).val.1).length := ⟨i.val, by rw [← h.right]; simp; rw [List.enum_with_lt_length_eq]; exact i.isLt⟩
+          exists i
+          rw [inductive_homomorphism_path_extends_prev]
+          rw [← ct.tree.getElem_children_eq_get_tree _ i']
+          simp only [← h.right]
+          simp
+          constructor
+          . rw [List.enum_with_lt_getElem_snd_eq_getElem]
+          . rw [List.enum_with_lt_getElem_fst_eq_index]
+        | inr ex_trg =>
+          apply Or.inr
+          unfold not_exists_trigger_opt_fs
+          unfold not_exists_trigger_list at ex_trg
+          constructor
+          . exact ex_trg.left
+          rw [inductive_homomorphism_path_extends_prev]
+          apply ct.tree.children_empty_means_all_following_none
+          exact ex_trg.right
+    fairness := by
+      intro trg
+      cases Classical.em (∃ n : Nat, nodes.infinite_list n ≠ none ∧ ∀ m : Nat, m > n -> nodes.infinite_list m = none) with
+      | inl h =>
+        cases h with | intro n hn =>
+          exists n
+          cases eq : nodes.infinite_list n with
+          | none => rw [eq] at hn; simp at hn
+          | some node =>
+            simp [Option.is_some_and]
+            constructor
+            . apply ct.fairness_leaves
+              unfold FiniteDegreeTree.leaves
+              unfold PossiblyInfiniteTree.leaves
+              simp only [Set.element]
+              exists (inductive_homomorphism_shortcut n).val.fst
+              constructor
+              . simp only [nodes, path] at eq; exact eq
+              . unfold PossiblyInfiniteList.empty
+                unfold PossiblyInfiniteTree.children
+                unfold InfiniteTreeSkeleton.children
+                simp
+                apply funext
+                have next_none := hn.right (n+1) (by simp)
+                have children_empty := inductive_homomorphism_tree_get_path_none_means_layer_empty n next_none
+                have all_none := ct.tree.children_empty_means_all_following_none _ children_empty
+                unfold FiniteDegreeTree.get at all_none
+                unfold PossiblyInfiniteTree.get at all_none
+                exact all_none
+            . intro m hm
+              have m_eq := hn.right m hm
+              simp only [nodes] at m_eq
+              rw [m_eq]
+              simp [Option.is_none_or]
+      | inr h =>
+        have h : ¬ ∃ n : Nat, nodes.infinite_list n = none := by
+          simp at h
+          simp
+          intro n
+          induction n with
+          | zero => simp [path, inductive_homomorphism_shortcut, inductive_homomorphism]; rw [ct.database_first]; simp
+          | succ n ih =>
+            specialize h n ih
+            cases h with | intro m hm =>
+              intro contra
+              have no_holes := nodes.no_holes m
+              simp only [nodes] at no_holes
+              specialize no_holes hm.right
+              cases Decidable.em ((n+1) = m) with
+              | inl eq => rw [eq] at contra; have contra' := hm.right; contradiction
+              | inr neq =>
+                let n_succ_fin_m : Fin m := ⟨n+1, by apply Nat.lt_of_le_of_ne; apply Nat.succ_le_of_lt; exact hm.left; exact neq⟩
+                specialize no_holes n_succ_fin_m
+                contradiction
+        cases ct.fairness_infinite_branches trg with | intro i hi =>
+          exists i
+          cases eq : nodes.infinite_list i with
+          | none => apply False.elim; apply h; exists i
+          | some node =>
+            constructor
+            . simp [Option.is_some_and]
+              specialize hi ((inductive_homomorphism_shortcut i).val.1) (by rw [(inductive_homomorphism_shortcut i).property.left]; simp)
+              simp only [nodes, path] at eq
+              rw [eq] at hi
+              simp [Option.is_none_or] at hi
+              exact hi
+            . intro j hj
+              specialize hi ((inductive_homomorphism_shortcut j).val.1) (by rw [(inductive_homomorphism_shortcut j).property.left]; apply Nat.le_of_lt; apply hj)
+              simp only [nodes, path]
+              exact hi
+  }
+  let result := branch.result
+
+  let global_h : GroundTermMapping sig := fun t =>
+    let dec := Classical.propDecidable (∃ f, f ∈ result ∧ t ∈ f.terms.toSet)
+    match dec with
+      | Decidable.isTrue p =>
+        let hfl := (Classical.choose_spec p).left
+        let i := Classical.choose hfl
+        let target_h := (inductive_homomorphism_shortcut i).val.2
+        target_h t
+      | Decidable.isFalse _ => t
+
+  have : ∀ i, (branch.branch.infinite_list i).is_none_or (fun chase_node => ∀ f, f ∈ chase_node.fact.val -> global_h.applyFact f = (inductive_homomorphism_shortcut i).val.snd.applyFact f) := by
+    intro i
+    cases eq : branch.branch.infinite_list i with
+    | none => simp [Option.is_none_or]
+    | some node =>
+      simp [Option.is_none_or]
+      intro f f_in_node
+      unfold GroundTermMapping.applyFact
+      simp [global_h]
+      intro t t_in_f
+      split
+      case h_2 _ n_ex _ =>
+        apply False.elim
+        apply n_ex
+        exists f
+        constructor
+        . have subset_result := chaseBranchSetIsSubsetOfResult branch i
+          rw [eq] at subset_result; simp [Option.is_none_or] at subset_result
+          apply subset_result
+          exact f_in_node
+        . rw [← List.listElementIffToSetElement]; exact t_in_f
+      case h_1 _ ex _ =>
+        let j := Classical.choose (Classical.choose_spec ex).left
+        let j_spec := Classical.choose_spec (Classical.choose_spec ex).left
+        cases Nat.le_total i j with
+        | inl i_le_j =>
+          have j_is_i_plus_k := Nat.le.dest i_le_j
+          cases j_is_i_plus_k with | intro k hk =>
+            simp [j] at hk
+            rw [← hk]
+            apply Eq.symm
+            simp only [inductive_homomorphism_shortcut]
+            have same_all_following := inductive_homomorphism_same_on_all_following_terms ct m m_is_model i
+            simp only [branch, path, inductive_homomorphism_shortcut] at eq
+            rw [eq] at same_all_following; simp [Option.is_none_or] at same_all_following
+            apply same_all_following
+            exact f_in_node
+            rw [← List.listElementIffToSetElement]; exact t_in_f
+        | inr j_le_i =>
+          have i_is_j_plus_k := Nat.le.dest j_le_i
+          cases i_is_j_plus_k with | intro k hk =>
+            rw [← hk]
+            simp only [inductive_homomorphism_shortcut]
+            have same_all_following := inductive_homomorphism_same_on_all_following_terms ct m m_is_model j
+            cases eq2 : branch.branch.infinite_list j with
+            | none => rw [eq2] at j_spec; simp [Option.is_some_and] at j_spec
+            | some _ =>
+              rw [eq2] at j_spec; simp [Option.is_some_and] at j_spec
+              simp only [branch, path, inductive_homomorphism_shortcut] at eq2
+              rw [eq2] at same_all_following; simp [Option.is_none_or] at same_all_following
+              apply same_all_following
+              exact j_spec
+              exact (Classical.choose_spec ex).right
+
+  exists result
+  exists global_h
+  constructor
+  . unfold ChaseTree.result
+    unfold Set.element
+    simp
+    exists branch
+    simp [result]
+    unfold ChaseTree.branches
+    unfold FiniteDegreeTree.branches
+    unfold PossiblyInfiniteTree.branches
+    unfold InfiniteTreeSkeleton.branches
+    unfold Set.element
+    simp
+    exists indices
+    intro n
+    simp only [path]
+    rw [indices_aux_result]
+    unfold FiniteDegreeTree.get
+    unfold PossiblyInfiniteTree.get
+    rfl
+  . constructor
+    . intro gt
+      split
+      case h_1 _ c =>
+        simp [global_h]
+        split
+        case h_1 _ p _ =>
+          let hfl := (Classical.choose_spec p).left
+          let i := Classical.choose hfl
+          let i_spec := Classical.choose_spec hfl
+          have property := (inductive_homomorphism_shortcut i).property.right
+          simp only [branch, path] at i_spec
+          cases eq : ct.tree.get (inductive_homomorphism_shortcut i).val.fst with
+          | none => rw [eq] at i_spec; simp [Option.is_some_and] at i_spec
+          | some node =>
+            rw [eq] at property; simp [Option.is_none_or] at property
+            exact property.left (GroundTerm.const c)
+        . trivial
+      . trivial
+    . intro f hf
+      simp only [result] at hf
+      unfold ChaseBranch.result at hf
+      unfold Set.element at hf
+      unfold GroundTermMapping.applyFactSet at hf
+      cases hf with | intro e he =>
+        let ⟨hel, her⟩ := he
+        simp [Set.element] at hel
+        cases hel with | intro n hn =>
+          rw [← her]
+          specialize this n
+          simp only [branch] at this
+          cases eq : path n with
+          | none => rw [eq] at hn; simp [Option.is_some_and] at hn
+          | some node =>
+            rw [eq] at hn; simp [Option.is_some_and] at hn
+            rw [eq] at this; simp [Option.is_none_or] at this
+            specialize this e hn
+            rw [this]
+            have property := (inductive_homomorphism_shortcut n).property.right
+            simp only [path] at eq
+            rw [eq] at property; simp [Option.is_none_or] at property
+            have : (inductive_homomorphism_shortcut n).val.snd.applyFactSet node.fact ⊆ m := property.right
+            unfold Set.subset at this
+            apply this
+            simp [Set.element, GroundTermMapping.applyFactSet]
+            exists e
+
